src/Init/Data/Array.lean
@@ -7,5 +7,4 @@ prelude
 import Init.Data.Array.Basic
 import Init.Data.Array.QSort
 import Init.Data.Array.BinSearch
-import Init.Data.Array.ForIn
 import Init.Data.Array.Macros
